MemTyp.v
@@ -1,0 +1,208 @@
+From Elo Require Import Util.
+From Elo Require Import Array.
+From Elo Require Import Core.
+From Elo Require Import CoreExt.
+
+From Elo Require Import Definitions.
+
+(* ------------------------------------------------------------------------- *)
+(* memtyp & uacc/sacc                                                        *)
+(* ------------------------------------------------------------------------- *)
+
+(* If there is access:
+   The access is unsafe if and only if the memtyp is mutable.
+*)
+Lemma memtyp_mut_iff_uacc : forall m t ad,
+  forall_memory m value ->
+  forall_memory m (consistently_typed_references m) ->
+  consistently_typed_references m t ->
+  access ad m t ->
+  (* --- *)
+  unsafe_access ad m t <-> (exists T, m[ad].typ = <{{&T}}>).
+Proof.
+  intros * ? ? ? Hacc. split.
+  - intros Huacc. clear Hacc. induction Huacc; inv_ctr; eauto.
+  - intros [? Heq]. induction Hacc; inv_ctr; eauto using unsafe_access.
+    + exfalso. eauto using nuacc_from_immutable_type.
+    + rewrite Heq in *. discriminate.
+Qed.
+
+(* If one access to an address is unsafe,
+   then all accesses to that address are unsafe.
+*)
+Corollary uacc_by_association : forall m t t' ad,
+  forall_memory m value ->
+  forall_memory m (consistently_typed_references m) ->
+  consistently_typed_references m t ->
+  consistently_typed_references m t' ->
+  (* --- *)
+  access ad m t ->
+  unsafe_access ad m t' ->
+  unsafe_access ad m t.
+Proof.
+  intros.
+  eapply memtyp_mut_iff_uacc; eauto.
+  eapply memtyp_mut_iff_uacc; eauto using uacc_then_acc.
+Qed.
+
+(* If there is access:
+   The access is safe if and only if the memtyp is immutable.
+*)
+Lemma memtyp_immut_iff_sacc : forall m t ad,
+  forall_memory m value ->
+  forall_memory m (consistently_typed_references m) ->
+  consistently_typed_references m t ->
+  access ad m t ->
+  (* --- *)
+  safe_access ad m t <-> (exists T, m[ad].typ = <{{i&T}}>).
+Proof.
+  intros * Hval ? ? Hacc. split.
+  - intros [? ?]. induction Hacc; invc_ctr; eauto; try inv_nuacc; eauto.
+    eapply IHHacc; eauto. intros ?. destruct (Hval ad'); inv_type; inv_uacc.
+  - intros [? Heq]; split; trivial.
+    induction Hacc; intros ?; invc_ctr; inv_uacc; eauto;
+    try (eapply IHHacc; eauto using uacc_by_association).
+    rewrite Heq in *. discriminate.
+Qed.
+
+(* If one access to an address is safe,
+   then all accesses to that address are safe.
+*)
+Corollary sacc_by_association : forall m t t' ad,
+  forall_memory m value ->
+  forall_memory m (consistently_typed_references m) ->
+  consistently_typed_references m t ->
+  consistently_typed_references m t' ->
+  (* --- *)
+  access ad m t ->
+  safe_access ad m t' ->
+  safe_access ad m t.
+Proof.
+  intros * ? ? ? ? ? Hsacc.
+  eapply memtyp_immut_iff_sacc; eauto.
+  specialize Hsacc as Hsacc'. destruct Hsacc' as [? ?].
+  eapply memtyp_immut_iff_sacc; eauto.
+Qed.
+
+(* ------------------------------------------------------------------------- *)
+(* memtyp preservation                                                       *)
+(* ------------------------------------------------------------------------- *)
+
+Module MemExt.
+  Reserved Infix "extends" (at level 20, no associativity).
+
+  Inductive extension : mem -> mem -> Prop :=
+    | extension_nil : forall m,
+      m extends nil
+
+    | extension_cons : forall m m' v v' T,
+      m extends m' ->
+      (cons (v, T) m) extends (cons (v', T) m') 
+
+    where " m 'extends' m' " := (extension m m').
+
+  Ltac nil_never_extends :=
+    match goal with
+    F : nil extends (cons _ _) |- _ => inv F
+    end.
+
+  Lemma refl : forall m,
+    m extends m.
+  Proof.
+    intros. induction m; eauto using extension.
+    match goal with |- (cons ?vT _) extends _ => destruct vT end.
+    eauto using extension.
+  Qed.
+
+  Lemma trans : forall m m' m'',
+    m  extends m'  ->
+    m' extends m'' ->
+    m  extends m''.
+  Proof.
+    intros * Hext **. generalize dependent m''.
+    induction Hext; intros; destruct m'';
+    eauto using extension; try nil_never_extends.
+    match goal with H : (cons _ _) extends (cons _ _) |- _ => inv H end.
+    eauto using extension.
+  Qed.
+
+  Lemma array_add : forall m vT,
+    (m +++ vT) extends m.
+  Proof.
+    intros. induction m; unfold Array.add; eauto using extension. simpl in *.
+    match goal with |- (cons ?vT _) extends _ => destruct vT end.
+    eauto using extension.
+  Qed.
+
+  Lemma array_get : forall m m' ad,
+    ad < #m' ->
+    m extends m' ->
+    m[ad].typ = m'[ad].typ.
+  Proof.
+    intros * Hlen Hext. generalize dependent ad. generalize dependent m.
+    induction m'; intros; try solve [inv Hlen].
+    destruct m; try nil_never_extends. invc Hext.
+    destruct ad; simpl; trivial. eauto using Arith.Lt.lt_S_n.
+  Qed.
+
+  Lemma array_set : forall m ad v T,
+    m[ad].typ = T -> 
+    m[ad <- (v, T)] extends m.
+  Proof.
+    intros. generalize dependent ad.
+    induction m; intros; eauto using extension. destruct ad;
+    match goal with |- _ extends (cons ?vT _) => destruct vT; subst end;
+    eauto using refl, extension.
+  Qed.
+
+  Lemma memext_mstep : forall m m' t t' e,
+    consistently_typed_references m t ->
+    m / t ==[e]==> m' / t' ->
+    m' extends m.
+  Proof.
+    intros. invc_mstep; eauto using refl, array_add.
+    eapply array_set. induction_tstep; intros; inv_ctr; eauto.
+    inv_ctr; trivial.
+  Qed.
+
+  Theorem memext_cstep : forall m m' ths ths' tid e,
+    forall_threads ths (consistently_typed_references m) ->
+    m / ths ~~[tid, e]~~> m' / ths' ->
+    m' extends m.
+  Proof.
+    intros. inv_cstep; eauto using refl, memext_mstep.
+  Qed.
+End MemExt.
+
+Theorem memtyp_cstep_preservation : forall m m' ths ths' tid e ad,
+  forall_threads ths (consistently_typed_references m) ->
+  (* --- *)
+  ad < #m ->
+  m / ths ~~[tid, e]~~> m' / ths' ->
+  m[ad].typ = m'[ad].typ.
+Proof.
+  symmetry. eauto using MemExt.array_get, MemExt.memext_cstep.
+Qed.
+
+(* ------------------------------------------------------------------------- *)
+(* memtyp inconsistency                                                      *)
+(* ------------------------------------------------------------------------- *)
+
+Lemma memtyp_inconsistency : forall m1 m2 t1 t2 ad,
+  forall_memory m1 value ->
+  forall_memory m2 value ->
+  forall_memory m1 (consistently_typed_references m1) ->
+  forall_memory m2 (consistently_typed_references m2) ->
+  consistently_typed_references m1 t1 ->
+  consistently_typed_references m2 t2 ->
+  (* --- *)
+  safe_access ad m1 t1 ->
+  unsafe_access ad m2 t2 ->
+  m1[ad].typ <> m2[ad].typ.
+Proof.
+  intros * ? ? ? ? ? Heq Hsacc Huacc.
+  eapply memtyp_immut_iff_sacc in Hsacc as [? Htyp1]; eauto using sacc_then_acc.
+  eapply memtyp_mut_iff_uacc   in Huacc as [? Htyp2]; eauto using uacc_then_acc.
+  rewrite Htyp1. rewrite Htyp2. discriminate.
+Qed.
+
