Safety.v
@@ -10,6 +10,7 @@ From Elo Require Import CoreExt.
 
 From Elo Require Import Definitions.
 
+From Elo Require Import MemTyp.
 From Elo Require Import PropertiesVAD.
 From Elo Require Import PropertiesACC.
 From Elo Require Import PropertiesUACC.
@@ -103,13 +104,13 @@ Theorem nacc_or_sacc_multistep_preservation : forall m m' ths ths' tid ad tc,
 Proof.
   intros * Hvp Hlt Hnacc **. induction_multistep; eauto.
   destruct (IHmultistep Hvp Hlt Hnacc) as [? | [? ?]]; subst.
-  - assert (valid_program m' ths') by eauto using vp_multistep_preservation. 
+  - assert (valid_program m' ths') by eauto using vp_preservation. 
     assert (#m <= #m')
       by eauto using multistep_monotonic_nondecreasing_memory_length.
     assert (ad < #m') by lia.
     eapply nacc_or_sacc_cstep_preservation in Hcstep as [? | [_ ?]]; subst;
     eauto with vp.
-  - assert (valid_program m' ths') by eauto using vp_multistep_preservation.
+  - assert (valid_program m' ths') by eauto using vp_preservation.
     assert (#m <= #m')
       by eauto using multistep_monotonic_nondecreasing_memory_length.
     assert (ad < #m') by lia.
@@ -118,60 +119,6 @@ Proof.
     decompose sum (lt_eq_lt_dec tid (#ths')); subst; trivial;
     simpl_array; inv_acc.
 Qed.
-
-Lemma something :
-  forall m1 m2 m3 m4 ths1 ths2 ths3 ths4 tid1 tid2 ad v1 v2 T tc,
-    valid_program m1 ths1 ->
-
-    forall_threads ths1 (valid_accesses m1) ->
-
-    ad < #m1 ->
-    ~ access ad m1 ths1[tid2] ->
-    access ad m3 ths3[tid2] ->
-    unsafe_access ad m1 ths1[tid1] ->
-
-    tid1 <> tid2 ->
-    m1 / ths1 ~~[tid1, EF_Write ad v1 T]~~> m2 / ths2 ->
-    m2 / ths2 ~~[tc]~~>* m3 / ths3 ->
-    m3 / ths3 ~~[tid2, EF_Read ad v2]~~> m4 / ths4 ->
-
-    False.
-Proof.
-  intros * ? ? ? ? ? Huacc ? Hcstep1 Hmultistep Hcstep2.
-
-  assert (valid_program m2 ths2) by eauto using vp_preservation. 
-  assert (valid_program m3 ths3) by eauto using vp_multistep_preservation. 
-  assert (#m1 <= #m2)
-    by eauto using cstep_monotonic_nondecreasing_memory_length.
-  assert (ad < #m2) by lia.
-  specialize Hcstep1 as Hcstep1'.
-  specialize Hmultistep as Hmultistep'.
-  eapply nacc_or_sacc_cstep_preservation in Hcstep1' as [? | [_ [? Hnuacc]]];
-  eauto with vp.
-  + eapply nacc_or_sacc_multistep_preservation
-      in Hmultistep' as [? | [? Hnuacc]];
-    eauto.
-    eapply memtyp_multistep_preservation in Hmultistep as Heq; eauto.
-    eapply memtyp_preservation in Hcstep1 as Heq'; eauto with vp.
-    rewrite Heq' in Heq.
-    eapply uacc_iff_memtyp_mut in Huacc as [? Hmt1];
-    eauto using uacc_then_acc with vp.
-    * eapply nuacc_iff_memtyp_immut in Hnuacc as [? Hmt2]; eauto with vp.
-      ** rewrite Hmt1 in Heq. rewrite Hmt2 in Heq. discriminate.
-      ** eapply des_vp_ctr. eauto. (* TODO *)
-    * eapply des_vp_ctr. eauto. (* TODO *)
-  + eapply memtyp_preservation in Hcstep1 as Heq; eauto with vp.
-    eapply uacc_iff_memtyp_mut in Huacc as [? Hmt1];
-    eauto using uacc_then_acc with vp.
-    * eapply nuacc_iff_memtyp_immut in Hnuacc as [? Hmt2]; eauto with vp.
-      ** rewrite Hmt1 in Heq. rewrite Hmt2 in Heq. discriminate.
-      ** eapply des_vp_ctr. eauto. (* TODO *)
-    * eapply des_vp_ctr. eauto. (* TODO *)
-Qed.
-
-(* ------------------------------------------------------------------------- *)
-(* TODO                                                                      *)
-(* ------------------------------------------------------------------------- *)
 
 Theorem safety : forall m m' ths ths' tid1 tid2 ad v1 v2 tc T,
   valid_program m ths ->
@@ -182,105 +129,45 @@ Theorem safety : forall m m' ths ths' tid1 tid2 ad v1 v2 tc T,
   False.
 Proof.
   intros * Hvp Hneq Hmultistep. specialize Hvp as H.
-  destruct H as [Hmval [[Hmwtt Hwtt] [[Hmvad Hvad] [[Hmctr Hctr] [Hss Hsms]]]]].
+  destruct H as [? [[? ?] [[? ?] [[? ?] [? Hsms]]]]].
   invc_multistep.
-
-  rename m'0 into m3. rename ths'0 into ths3.
-  rename H6 into Hmultistep. rename H7 into Hcstep.
+  (* some renamings to make the hypotheses readable *)
   match goal with
-  | H1 : _ / _ ~~[ _    ]~~>* _ / _
-  , H2 : _ / _ ~~[ _, _ ]~~>  _ / _
+  | H1 : ?m / ?ths ~~[ _    ]~~>* ?m' / ?ths'
+  , H2 : _  / _    ~~[ _, _ ]~~>  _   / _
   |- _ =>
-    rename H1 into Hmultistep; rename H2 into H3_cstep
+    rename m into m1; rename ths into ths1;
+    rename m' into m3; rename ths' into ths3;
+    eapply destruct_multistep in H1 as [m2 [ths2 [Hcstep1___ Hmultistep]]];
+    move H2 after Hmultistep; rename H2 into Hcstep2___
   end.
-
-  assert (Hacc' : access ad m3 ths3[tid2])
-    by eauto using cstep_read_requires_acc.
-  eapply destruct_multistep in Hmultistep
-    as [m2 [ths2 [H1_cstep H2_multistep]]].
-  assert (Huacc : unsafe_access ad m ths[tid1])
-    by eauto using cstep_write_requires_uacc.
-  destruct (acc_dec ad m ths[tid2]) as [? | Hnacc];
-  try solve [eapply (Hsms tid1 tid2); eauto].
-  assert (Hvac : forall_threads ths (valid_accesses m))
+  (* --- *)
+  assert (Hvac : forall_threads ths1 (valid_accesses m1))
     by (intros ?; eauto using vad_then_vac).
-  assert (Hlen1 : ad < #m)
+  assert (valid_program m2 ths2) by eauto using vp_preservation. 
+  assert (valid_program m3 ths3) by eauto using vp_preservation. 
+  (* --- *)
+  assert (#m1 <= #m2)
+    by eauto using cstep_monotonic_nondecreasing_memory_length.
+  assert (ad < #m1)
     by eauto using vac_length, cstep_write_requires_uacc, uacc_then_acc.
-
-  eapply something; eauto.
+  assert (ad < #m2) by lia.
+  (* --- *)
+  assert (Hacc : access ad m3 ths3[tid2])
+    by eauto using cstep_read_requires_acc.
+  assert (Huacc : unsafe_access ad m1 ths1[tid1])
+    by eauto using cstep_write_requires_uacc.
+  assert (Hnacc : ~ access ad m1 ths1[tid2])
+    by (intros ?; eapply (Hsms tid1 tid2); eauto).
+  (* --- *)
+  assert (m1[ad].typ = m2[ad].typ) as HeqA by eauto using memtyp_preservation.
+  eapply nacc_or_sacc_cstep_preservation in Hcstep1___ as [? | [_ Hsacc]];
+  eauto with vp.
+  + assert (m2[ad].typ = m3[ad].typ) as HeqB by eauto using memtyp_preservation.
+    eapply nacc_or_sacc_multistep_preservation in Hmultistep as [? | Hsacc];
+    eauto.
+    rewrite HeqB in HeqA.
+    eapply (memtyp_inconsistency m3 m1 ths3[tid2] ths1[tid1]); eauto with vp.
+  + eapply (memtyp_inconsistency m2 m1 ths2[tid2] ths1[tid1]); eauto with vp.
 Qed.
 
-(* ------------------------------------------------------------------------- *)
-(* TODO                                                                      *)
-(* ------------------------------------------------------------------------- *)
-
-(*
-Lemma access_granted_by_alloc_is_memory_length : forall m t t' ad v Tr,
-  ~ access ad m t ->
-  t --[EF_Alloc (#m) v Tr]--> t' ->
-  access ad (m +++ (v, Tr)) t' ->
-  ad = length m.
-Proof.
-  intros * Hnacc ? Hacc.
-  induction_tstep; inv_nacc; inv_acc; eauto using access.
-  - match goal with F : access _ _ _ |- _ => contradict F end.
-    simpl_array. eapply access_add; eauto.
-  - do 2 auto_specialize. eapply IHstep.
-    eapply acc_asg in Hacc as [? | ?]; eauto.
-    exfalso. eapply (not_access_allocated_value _ l) in HnaccL; eauto. 
-    eapply (access_add _ r); eauto.
-  - eapply asg_access_inverse in Hnacc as [? HnaccR].
-    match goal with IH : _ -> _ -> _ -> ?x |- ?x => eapply IH; eauto end.
-    eapply asg_access in Hacc as [? | ?]; eauto.
-    exfalso. eapply (not_access_allocated_value _ r) in HnaccR; eauto. 
-    eapply (access_add _ l); eauto.
-  - eapply seq_access_inverse in Hnacc as [HnaccT1 ?].
-    match goal with IH : _ -> _ -> _ -> ?x |- ?x => eapply IH; eauto end.
-    eapply seq_access in Hacc as [? | ?]; eauto.
-    exfalso. eapply (not_access_allocated_value _ t1) in HnaccT1; eauto. 
-    eapply (access_add _ t2); eauto.
-Qed.
-
-Theorem access_needs_alloc : forall m m' t t' eff ad,
-  ~ access m t ad ->
-  m / t ==[eff]==> m' / t' ->
-  access m' t' ad ->
-  exists v, eff = (EF_Alloc ad v).
-Proof.
-  intros * Hnacc Hmstep Hacc. inversion Hmstep; subst.
-  - contradict Hacc. eauto using none_does_not_grant_access.
-  - eexists. erewrite <- access_granted_by_alloc_is_memory_length; eauto.
-  - contradict Hacc. eauto using load_does_not_grant_access.
-  - contradict Hacc. eauto using store_does_not_grant_access.
-Qed.
-
-Theorem access_needs_alloc_multistep : forall m m' t t' ad tc,
-  ~ access m t ad ->
-  m / t ==[tc]==>* m' / t' ->
-  access m' t' ad ->
-  exists v, In (EF_Alloc ad v) tc.
-Proof.
-  intros * Hnacc Hmultistep Hacc.
-  induction Hmultistep; try solve [exfalso; eauto].
-  destruct (access_dec m' t' ad) as [Hacc' | ?].
-  - destruct (IHHmultistep Hnacc Hacc').
-    eexists. right. eauto.
-  - assert (Heq : exists v, eff = EF_Alloc ad v);
-    eauto using access_needs_alloc.
-    destruct Heq. eexists. left. eauto.
-Qed.
-*)
-
-(*
-
-(* PART 6 *)
-
-Theorem concurrent_duplicate_alloc :
-  forall m m' ths ths' tid tid' tc1 tc2 ad v v',
-  ~ (m / ths ~~[tc1 ++ (tid , EF_Alloc ad v ) ::
-                tc2 ++ (tid', EF_Alloc ad v') :: nil]~~>* m' / ths').
-Proof.
-  intros * F. inversion F; subst; clear F.
-Abort.
-
-*)
